tree/local.v
@@ -7,6 +7,10 @@ Import ListNotations.
 Require Import Morphisms.
 Require Import Lia.
 
+(* coinduction by Pous *)
+(* From Coinduction Require Import all. Import CoindNotations.
+Set Implicit Arguments. *)
+
 CoInductive ltt: Type :=
   | ltt_end : ltt
   | ltt_recv: part -> list (option(sort*ltt)) -> ltt
@@ -81,7 +85,91 @@ Inductive subtype (R: ltt -> ltt -> Prop): ltt -> ltt -> Prop :=
                     wfsend subsort R xs ys ->
                     subtype R (ltt_send p xs) (ltt_send p ys).
 
+Check gpaco2.
+
 Definition subtypeC l1 l2 := paco2 subtype bot2 l1 l2.
+
+Lemma monoR: forall xs ys R1 R,
+  (forall a a0 : ltt, R1 a a0 -> R a a0) ->
+   wfrec subsort R1 ys xs ->
+   wfrec subsort R ys xs.
+Proof. intro xs.
+       induction xs; intros.
+       - case_eq ys; intros.
+         + simpl. easy.
+         + subst. simpl in H0. easy.
+       - case_eq ys; intros.
+         + subst. easy.
+         + subst. simpl in H0.
+           destruct o. destruct p, a. destruct p.
+           simpl. split. easy. split. apply H. easy.
+           apply IHxs with (R1 := R1).
+           easy. easy.
+           easy.
+           simpl. 
+           destruct a. easy.
+           apply IHxs with (R1 := R1). easy.
+           easy.
+Qed.
+
+(* Lemma monoS: forall xs ys R1 R,
+  (forall a a0 : ltt, R1 a a0 -> R a a0) ->
+   wfsend subsort R1 xs ys ->
+   wfsend subsort R xs ys.
+Proof. intro xs.
+       induction xs; intros.
+       - case_eq ys; intros.
+         + simpl. easy.
+         + subst. simpl in H0. easy.
+       - case_eq ys; intros.
+         + subst. easy.
+         + subst. simpl in H0.
+           destruct o. destruct p, a. destruct p.
+           simpl. split. easy. split. apply H. easy.
+           apply IHxs with (R1 := R1).
+           easy. easy.
+           easy.
+           simpl. 
+           destruct a. easy.
+           apply IHxs with (R1 := R1). easy.
+           easy.
+Qed.
+
+Definition bst: mon (ltt -> ltt -> Prop).
+Proof. unshelve econstructor.
+       - intros R t1 t2.
+         exact (subtype R t1 t2).
+       - cbv. intros R1 R2 leqR x y HR1.
+         induction HR1. 
+         + constructor.
+         + constructor. apply monoR with (R1 := R1); easy.
+         + constructor. apply monoS with (R1 := R1); easy.
+Defined.
+ *)
+(* Program Definition b: mon (ltt -> ltt -> Prop) :=
+   {| body R s t := subtype R s t |}.
+ Next Obligation.
+  cbv. intros R1 R CIH a b H. 
+  induction H. constructor. 
+  constructor.
+  apply monoR with (R1 := R1).
+  easy. easy.
+  
+  constructor.
+  apply monoS with (R1 := R1).
+  easy. easy.
+Qed. *)
+
+(* Print mon.
+Print gfp.
+Print inf'.
+Print mon.
+Print CompleteLattice.
+
+Infix "⩽" := (gfp bst) (at level 70).
+Notation "x ⩽[ R ] y" := (`R x y) (at level 79).
+(* Notation "x ≃ y" := (`_ x y) (at level 79). *)
+Notation "x [⩽] y" := (bst `_ x y) (at level 79). *)
 
 Lemma trans_recv: forall (l1 l2 l3:  list (option(sort*ltt))) (R1: sort -> sort -> Prop) (R2: ltt -> ltt -> Prop),
    Transitive R1 -> Transitive R2 ->
@@ -217,11 +305,101 @@ Proof. pcofix CIH.
 Qed.
 
 Lemma stTransH: forall l1 l2 l3 R, Transitive R -> subtype R l1 l2 -> subtype R l2 l3 -> subtype R l1 l3.
-Proof. Admitted.
+Proof. intros.
+       
+       induction H0.
+       induction H1.
+       constructor.
+       constructor. easy.
+       constructor. easy.
+       
+       case_eq l3; intros.
+       subst. inversion H1. subst.
+       inversion H1. subst.
+       constructor.
+       apply trans_recv with (l2 := ys).
+       repeat intro.
+       apply sstrans with (s2 := y); easy.
+       easy. easy. easy.
+       subst. inversion H1.
+       
+       case_eq l3; intros.
+       subst. inversion H1.
+       subst.
+       inversion H1. subst.
+       inversion H1. subst.
+       
+       
+       constructor.
+       apply trans_send with (l2 := ys). 
+       repeat intro.
+       apply sstrans with (s2 := y); easy.
+       easy. easy. easy.
+Qed.
+
+#[export] Instance Transitive_st {R} {HR: Transitive R}: Transitive (subtype R).
+Proof. repeat intro.
+       induction H0.
+       induction H.
+       constructor.
+       constructor. easy.
+       constructor. easy.
+
+       case_eq x; intros.
+       subst. inversion H.
+       subst. inversion H. subst.
+       constructor.
+       apply trans_recv with (l2 := xs).
+       repeat intro.
+       apply sstrans with (s2 := y); easy.
+       easy. easy. easy.
+       subst. inversion H.
+
+       case_eq x; intros.
+       subst. inversion H.
+       subst. inversion H. 
+       subst. inversion H. subst.
+
+       constructor.
+       apply trans_send with (l2 := xs). 
+       repeat intro.
+       apply sstrans with (s2 := y); easy.
+       easy. easy. easy.
+Qed.
+
+(* #[export] Instance Transitive_t: forall {R: Chain bst}, Transitive `R.
+Proof. apply Transitive_chain.
+       intros R HR.
+       assert (H: forall x y z, bst `R x y -> bst `R y z -> bst `R x z).
+       { intros.
+         case_eq x; case_eq y; case_eq z; intros; try (subst; easy).
+         subst. inversion H. subst. inversion H0. subst.
+         constructor.
+         apply trans_recv with (l2 := l0).
+         repeat intro.
+         apply sstrans with (s2 := y); easy.
+         easy. easy. easy.
+
+         subst. inversion H. subst. inversion H0. subst.
+         constructor.
+         apply trans_send with (l2 := l0).
+         repeat intro.
+         apply sstrans with (s2 := y); easy.
+         easy. easy. easy.
+       }
+       intros x y z xy yz.
+       apply H with (y := y); easy.
+Qed.
+
+Lemma stTransPous: forall t1 t2 t3, t1 ⩽ t2 -> t2 ⩽ t3 -> t1 ⩽ t3.
+Proof. intros.
+    (* rewrite <- H0; exact H. *)
+       apply transitivity with (y := t2); easy.
+Qed. *)
+
 
 Lemma stTrans: forall l1 l2 l3, subtypeC l1 l2 -> subtypeC l2 l3 -> subtypeC l1 l3.
 Proof. Admitted.
- 
 
 (* #[export]
 Declare Instance stTrans: Transitive (subtypeC).
